---
layout: post
title: My Take on Haskell#1
excerpt-separator: <!---->
---

Haskell is a functional programming language. Why do you need to know about it? Because you should.

<!---->

The utilities you should have once Haskell is setup on your PC.

> ghc, ghci and cabal \
> Load a script with functions with `:l <fileName>`

Pure functions, Immutable Data
So **no** side effects

Declarative
Easier to verify correctness  
Definition of complex enough algorithms can be done elegantly in Haskell.  
Note that I have learnt that examples help in understanding a lot more than definitions by themselves. So including a tonne of them.

## Function Definition

```hs
name arg1 arg2 arg3 = < exp >
```

There is no return statement. The last statement evaluated is returned

## Types

`var :: Type`  
e.g. x :: Integer  
`func :: Type`  
e.g. inRange :: Integer -> Integer -> Integer -> Bool

### Let

Imperative isn't allowed, i.e. you can't return a value.
So instead, we use `let`

```hs
func params =
    let params = < exp >
    in params
```

That is, we define a name, and bind it to an expression, i.e. some name and expression, another name and it's expression...and finally `in` and all "bind-ed" expression containing all names

> Things are evaluated only when needed, Lazy Haskell

### Where

```hs
func params = paramsToBeReturned --technically not "returned"
    where
    params = < exp >
```

### if-then-else

```hs
if < exp > then < exp > else < exp >
```

## Infix Functions

```hs
:t (+) --for checking type of any function
> (+) :: Num a=>a->a->a
```

Any function can be written in Infix style by \` \` around them

## Recursion

No loops in Haskell. So we need recursion

```hs
fac n =
    if n <= 1 then
        1
    else
        n * fac (n-1)
```

### Guards

> `otherwise` always evaluates to True

Guards can replace if-then-else, as that guard is executed, and returned as THE expression of the function which evaluates to True

```hs
fac n
    | n <= 1 = 1
    | otherwise = n*fac(n-1)
```

```
    | < exp to be evaluated for True or False > = < exp returned >
```

> `_` is a wild card

## Pattern Matching

Multiple definitions of the same functions can occur in Haskell, each with different set of inputs

```
ghci> is_zero 0 = True
...
ghci> is_zero _ = False
```

This means that for 0, is_zero will return True, and for a wild card "Excluding the already defined input set", the function returns False

### Accumulators

```hs
fac n = aux n 1 --aux is an auxiliary function, which takes an accumulator
    where
        aux n acc --definition of aux
         | n <= 1 = acc
         | otherwise = aux (n - 1) (n * acc)
```

In short, accumulators are applying Tail Recursion.  
This is much more efficient than usual recursion, cause it takes a lot less memory and same complexity.  
The main thing to remember about tail recursion is that the recursive step is always the last step at a particular depth.

Another example on Fibonacci

```hs
fib n = go n (a, b)
    where
        go 0 (a, b) = a
        go 1 (a, b) = b
        go n (a, b) = go (n-1) (b, a + b)
```

## Lists

Lists only have one internal type. They can be constructed via constructors `[]` (empty) and `:` (pre-pend)

example:

```hs
asc :: Int -> Int -> [Int]
asc n m --list from n to m
    | m < n = []
    | m == n = [m]
    | m > n = n : asc (n+1) m
```

Many functions of Lists are predefined, quite a lot of them in `Data.List` module.

#### For Polymorphic Lists:

```hs
elem :: a -> [a] -> Bool --returns if given element belongs to the list
head :: [a] -> a --returns the first element of the list
tail :: [a] -> a --returns all of list except the head
length :: [a] -> Int --returns length of list
init :: [a] -> [a] --returns a last-element-removed list
last :: [a] -> a --returns the last element of list
null :: [a] -> Bool --check if a list is empty
```

Every data structure in Haskell is immutable, so we always get a copy with modifications to current structure, which we may reassign to the same variable name, that effectively changes the data structure.

#### For Boolean Lists:

```hs
and :: [Bool] -> Bool --and operation over all elements of list
or :: [Bool] -> Bool --or operation over all elements of list
```

When can such a thing be useful, a list of booleans?  
The case of List Comprehensions.

## List Comprehension

```
[<gen> | <elem> <- <list>, ... , <guard>, ... ]
```

#### Patterns in Lists

Pattern matching with Lists is quite useful. It is used mostly in recursion tbh

```hs
sum [] = 0
sum (x:xs) = x + sum xs
-- is equivalent to
sum xs = foldr (+) 0 xs

-- another example
evens :: [Int] -> [Int]
evens [] = []
evens (x:xs) --colon constructor
    | mod x 2 == 0 = x : evens xs
    | otherwise = evens xs
```

## Tuples

Tuples can have any number of elements, but a fixed number

```hs
fst :: (a,b) -> a
fst (x,_) = x

snd :: (a,b) -> b
snd (_,y) = y
```

#### Tuple "unpacking"

`let (x, y) = (1, 2) in x`

### Higher Order Functions

```hs
app :: (a -> b) -> a -> b
app f x = f x
add1 :: Int -> Int
add1 x = x + 1
app add1 1
```

#### Anonymous Functions

(\\\<args> -> \<expr>)

example `(\x -> x+1)`  
Functions are just values in Haskell, just like Js, can be assigned to variables

```hs
increment = (\x -> x+1)
addAll = (\x y z -> x+y+z)

app f x = f x
incrementOne = app (\x -> x + 1) 1
```

#### Some common Higher order functions

```hs
-- Map is useful to map each element of a list to another list via a function
map :: (a->b) -> [a] -> [b]
map (\(x,y) -> x+y) [(1,2),(2,3),(4,6)]

-- Filter is used to filter out a list on the basis of a provided function
-- this is a predicate function
-- the predicate when returns True, then the element will be in the new list
filter :: (a->Bool) -> [a] -> [a]
filter (\x -> x>2) [1,2,3,4,5,6]
filter (\(x,y) -> x/=y) [(1,2),(2,2)]
```

### Currying

Essentially, functions having multiple arguments don't exist.
`f :: a -> b -> c -> d` is equivalent to `f :: a -> (b -> (c -> d))`

So, example:

```hs
add :: Int -> Int -> Int
add x y = x + y
-- or equivalent to
add x = (\y -> x+y)
-- or equivalent to
add = (\x -> (\y -> x + y))
-- so clearly, anonymous functions are fundamental, while any function itself is just a variable which has an anonymous function assigned to it.

add 1 -- returns a function
add 1 :: Int -> Int
```

The last statement is generating a new function from an old function. This is called the **partial function application**.

This is done everywhere in Haskell. Example, you might use a map or filter (higher order functions), but have to rewrite it's filtering function every time. Partial function application is a way out.

```hs
doubleList = map (\x -> 2*x)
-- now we don't need any function argument to do this operation. Just pass a list, and doubleList will double it element wise ofc
```

## Function Composition

Haskell is great for implementing mathematical functions, and its exactly that.

```hs
(.) :: (b -> c) -> (a -> b) -> a -> c
f :: a -> b
g :: a -> b
composite f g = f.g
composite f g = (\x -> f (g x))
```

Application? If you have a sorting function `sort` and reverting function `reverse`, define

```hs
descSort = reverse.sort
descSort = (\x -> reverse (sort x))
descSort x = reverse (sort x)
-- All are equivalent
```

Another example, mapping of mappings

```hs
map2D :: (a->b) -> [[a]] -> [[b]]
map2D = map.map
```

#### $ function

Used to write cleaner code while using composition or higher order functions

```hs
($) :: (a -> b) -> (a -> b)
f $ x = f x
-- or
($) f x = f x
-- or
($) = id
```

Applications:

```hs
f xs = map (\x -> x+1) (filter (\x -> x>1) xs)
-- or
f xs = map (\x -> x+1) $ filter (\x -> x>1) xs
```

## Folding

One of the most important concept in Lists. Folding up a list's element into a value, on the basis of a binary function and an initiator (accumulator)

```hs
foldr :: (a -> b -> b) -> b -> [a] -> b
foldr (\elem acc -> <term>) <start_acc> <list>

foldr (%) a [x1, x2, x3, x4] = x1 % x2 % x3 % x4 % a
-- a is accumulator, % is a binary function
```

Applications:

```hs
-- some partial functions
sum = foldr (+) 0
and = foldr (&&) True
or = foldr (||) False
length = foldr (\x -> (+) 1) 0
length' = foldr (const $ (+) 1) 0 -- as x isn't used, replace it by const
map f = foldr ((:) . f) []

count x = foldr (\y acc -> if x==y then acc+1 else acc) 0 -- a partial function that counts how many times an element occurs in a list
isAll e = foldr (\x acc -> e==x && acc) True -- note that this isn't efficient, but that's not the point
isAll' e = foldr (\x -> (&&) $ e == x) True
```

Now, folding has direction. We have seen `foldr`, and there exists a `foldl`

```hs
foldr (\elem acc -> <term>) <start_acc> <list> --from last element of list with the acc, we build upto the first
foldl (\acc elem -> <term>) <start_acc> <list> --from the first element with the acc, we build upto the last
```

#### Tree folding

In a Lazy based language, the order of folding of trees actually shouldn't matter.  
But while printing, we need to take order into account.

## Data Types

```hs
data Name =
    Constructor1 <args> | Constructor2 <args> | ..
    -- args shouldn't contain literals, but the type itself
```

```hs
data Color =
    Red | Green | Blue

data PeaNum =
    Succ PeaNum | Zero

data Calculation =
    Add Int Int | Mul Int Int | Sub Int Int | Div Int Int

data Tree a =
    Leaf | Node (Tree a) a (Tree a)
    -- specifying a is necessary cause a tree should have a particular datatype stored
```

Using the above defined data-types

```hs
-- using the custom datatype Calculation
calc :: Calculation -> Int
calc (Add x y) = x+y
calc (Sub x y) = x-y
calc (Mul x y) = x*y
calc (Div x y) = x/y


tree :: Tree Int
tree = Node (Node Leaf 1 Leaf) 2 (Node (Node Leaf 3 Leaf) 4 Leaf)

-- recursive data-type
add :: PeaNum -> PeaNum -> PeaNum
add Zero n = n
add (Succ m) n = Succ (add m n)

sum :: [PeaNum] -> PeaNum
sum [] = Zero
sum (x:xs) = add x (sum xs)
```

All mighty reference link, an interactive guide:
[http://learnyouahaskell.com/](http://learnyouahaskell.com/)

### This is a summary/writeup of Lessons by _Philipp Hagenlocher_.
